Simplifying the language (a lot)

Safety.v
@@ -1,60 +1,106 @@
+From Coq Require Import Arith.Arith.
+From Coq Require Import Lists.List.
+From Coq Require Import Logic.ClassicalFacts.
 
+From Elo Require Export Core0.
 
-From Elo Require Export Core.
+Reserved Notation "m / t / tc '==>*' m' / t' / tc'"
+  (at level 40, t at next level, tc at next level,
+                m' at next level, t' at next level).
 
-Inductive has_access : tm -> nat -> Prop :=
-  | has_access_trans : forall ad ad' m t,
+Definition trace := list effect.
+
+Inductive has_access (m : mem) : tm -> addr -> Prop :=
+  | has_access_trans : forall t ad ad',
     get_tm m ad = TM_Loc ad' ->
-    has_access t ad ->
-    has_access t ad'
-
-  | has_access_fun : forall ad p P block R,
-    has_access block ad ->
-    has_access (TM_Fun p P block R) ad
-
-  | has_access_new : forall ad t,
-    has_access t ad ->
-    has_access (TM_New t) ad
+    has_access m t ad ->
+    has_access m t ad'
 
   | has_access_loc : forall ad,
-    has_access (TM_Loc ad) ad
+    has_access m (TM_Loc ad) ad
 
-  | has_access_load : forall ad t,
-    has_access t ad ->
-    has_access (TM_Load t) ad
+  | has_access_new : forall t ad,
+    has_access m t ad ->
+    has_access m (TM_New t) ad
 
-  | has_access_asg1 : forall ad l r,
-    has_access l ad ->
-    has_access (TM_Asg l r) ad
+  | has_access_load : forall t ad,
+    has_access m t ad ->
+    has_access m (TM_Load t) ad
 
-  | has_access_asg2 : forall ad l r,
-    has_access r ad ->
-    has_access (TM_Asg l r) ad
+  | has_access_asg1 : forall l r ad,
+    has_access m l ad ->
+    has_access m (TM_Asg l r) ad
 
-  | has_access_call1 : forall ad f a,
-    has_access f ad ->
-    has_access (TM_Call f a) ad
-
-  | has_access_call2 : forall ad f a,
-    has_access a ad ->
-    has_access (TM_Call f a) ad
-
-  | has_access_seq1 : forall ad t1 t2,
-    has_access t1 ad ->
-    has_access (TM_Seq t1 t2) ad
-
-  | has_access_seq2 : forall ad t1 t2,
-    has_access t2 ad ->
-    has_access (TM_Seq t1 t2) ad
-
-  | has_access_let1 : forall ad id E e t,
-    has_access e ad ->
-    has_access (TM_Let id E e t) ad
-
-  | has_access_let2 : forall ad id E e t,
-    has_access t ad ->
-    has_access (TM_Let id E e t) ad
+  | has_access_asg2 : forall l r ad,
+    has_access m r ad ->
+    has_access m (TM_Asg l r) ad
   .
+
+Theorem aux1 : forall m t t' ad v,
+  t' --[EF_Alloc ad v]--> t ->
+  has_access m t ad.
+Proof.
+  intros ? ? ?. generalize dependent t.
+  induction t'; intros * Hstep;
+  inversion Hstep; eauto using has_access.
+Qed.
+
+Inductive multistep : mem -> tm -> trace -> mem -> tm -> trace -> Prop :=
+  | multistep_first : forall main ad,
+    ~ (has_access nil main ad) ->
+    nil / TM_Nil / nil ==>* nil / main / (EF_None :: nil)
+
+  | multistep_step : forall m m' m'' t t' t'' tc tc' ceff,
+    m  / t / tc ==>* m' / t' / tc' ->
+    m' / t' ==[ceff]==> m'' / t'' ->
+    m  / t / tc ==>* m'' / t'' / (ceff :: tc')
+
+  where "m / t / tc '==>*' m' / t' / tc'" := (multistep m t tc m' t' tc').
+
+
+
+
+
+
+
+
+
+
+Lemma ceff_eq_dec : forall (x y : ceffect),
+  x = y \/ x <> y.
+Admitted.
+
+Theorem todo : forall m_ m ths_ ths tc_ tc tid ad v,
+  m_ / ths_ / tc_ ==>* m / ths / (CEF_Load tid ad v :: tc) ->
+  In (CEF_Alloc tid ad v) tc.
+Proof.
+  intros * Hmstep.
+  inversion Hmstep. subst.
+
+
+
+
+induction tc as [| ceff tc' IH].
+  - inversion Hmstep; subst. inversion H6.
+  - destruct (ceff_eq_dec ceff (CEF_Alloc tid ad v)); subst.
+    + eapply in_eq.
+    + eapply in_cons. clear H.
+      inversion Hmstep. subst.
+      inversion H6; subst.
+      * shelve.
+      *
+
+
+      inversion Hmstep. subst. clear Hmstep.
+      induction H7.
+      * inversion H8. subst.
+      eapply IH. clear IH.
+
+Qed.
+
+
+
+
 
 (*
 
