Core0.v
@@ -1,0 +1,151 @@
+From Coq Require Import Init.Nat.
+From Coq Require Import List.
+
+From Elo Require Export Array.
+From Elo Require Export Map.
+
+Import ListNotations.
+
+Definition name := String.string.
+Definition num := nat.
+
+(* Notations *)
+
+Reserved Notation "t '--[' eff ']-->' t'"
+  (at level 40).
+Reserved Notation "m / ths '==[' ceff ']==>' m' / ths'"
+  (at level 40, ths at next level, ceff at next level, m' at next level).
+Reserved Notation "mt / Gamma '|--' t 'is' T"
+  (at level 40, Gamma at next level).
+
+(* Types *)
+
+Inductive typ : Set :=
+  | TY_Void
+  | TY_Num
+  | TY_Ref : typ -> typ
+  .
+
+(* Terms *)
+
+Inductive tm : Set :=
+  | TM_Nil
+  | TM_Num  : num -> tm
+  | TM_Loc  : num -> tm
+  | TM_New  : tm -> tm
+  | TM_Load : tm -> tm
+  | TM_Asg  : tm -> tm -> tm
+  .
+
+(* Values *)
+
+Inductive value : tm -> Prop :=
+  | V_Nil : value TM_Nil
+  | V_Num : forall n, value (TM_Num n)
+  | V_Loc : forall i, value (TM_Loc i)
+  .
+
+(* Effects *)
+
+Definition addr := nat.
+
+Inductive effect : Set :=
+  | EF_None
+  | EF_Alloc (ad : addr) (t : tm)
+  | EF_Load  (ad : addr) (t : tm)
+  | EF_Store (ad : addr) (t : tm)
+  .
+
+(* Auxiliary Aliases *)
+
+Definition ctx := map typ.
+Definition mem := list tm.
+(* Definition threads := list tm. *)
+Definition memtyp := list typ.
+Definition get_typ := get TY_Void.
+Definition get_tm  := get TM_Nil.
+Definition get_ctx := get (@empty typ).
+
+(* Operational Semantics *)
+
+Local Infix "=?" := String.eqb (at level 70, no associativity).
+
+Inductive step : tm -> effect -> tm -> Prop :=
+  (* New *)
+  | ST_New1 : forall t t' eff,
+    t --[eff]--> t' ->
+    TM_New t --[eff]--> t'
+
+  | ST_New : forall t ad,
+    value t ->
+    TM_New t --[EF_Alloc ad t]--> TM_Loc ad
+
+  (* Load *)
+  | ST_Load1 : forall t t' eff,
+    t --[eff]--> t' ->
+    TM_Load t --[eff]--> TM_Load t'
+
+  | ST_Load : forall ad t,
+    TM_Load (TM_Loc ad) --[EF_Load ad t]--> t
+
+  (* Asg *)
+  | ST_Asg1 : forall l l' r eff,
+    l --[eff]--> l' ->
+    TM_Asg l r --[eff]--> TM_Asg l' r
+
+  | ST_Asg2 : forall l r r' eff,
+    value l ->
+    r --[eff]--> r' ->
+    TM_Asg l r --[eff]--> TM_Asg l r'
+
+  | ST_Asg : forall t ad,
+    value t ->
+    TM_Asg (TM_Loc ad) t --[EF_Store ad t]--> TM_Nil
+
+  where "t '--[' eff ']-->' t'" := (step t eff t').
+
+(* Memory Step *)
+
+Inductive mstep : mem -> tm -> effect -> mem -> tm -> Prop :=
+  | MST_Alloc : forall m t t' v,
+    t --[EF_Alloc (length m) v]--> t' ->
+    m / t ==[ EF_Alloc (length m) v ]==> (add m v) / t'
+
+  | MST_Load : forall m t t' ad,
+    t --[EF_Load ad (get_tm m ad)]--> t' ->
+    m / t ==[ EF_Load ad (get_tm m ad) ]==> m / t'
+
+  | MST_Store : forall m t t' ad v,
+    ad < length m ->
+    t --[EF_Store ad v]--> t' ->
+    m / t ==[ EF_Store ad v ]==> (set m ad v) / t'
+
+  where "m / t '==[' eff ']==>' m' / t'" := (mstep m t eff m' t').
+
+(* Typing *)
+
+Inductive well_typed_term (mt : memtyp) : ctx -> tm -> typ -> Prop :=
+  | T_Nil : forall Gamma,
+    mt / Gamma |-- TM_Nil is TY_Void
+
+  | T_Num : forall Gamma n,
+    mt / Gamma |-- (TM_Num n) is TY_Num
+
+  | T_Loc : forall Gamma ad,
+    ad < length mt ->
+    mt / Gamma |-- (TM_Loc ad) is TY_Ref (get_typ mt ad)
+
+  | T_New : forall Gamma t T,
+    mt / Gamma |-- t is T ->
+    mt / Gamma |-- (TM_New t) is (TY_Ref T)
+
+  | T_Load : forall Gamma t T,
+    mt / Gamma |-- t is TY_Ref T ->
+    mt / Gamma |-- (TM_Load t) is T
+
+  | T_Asg : forall Gamma l r T,
+    mt / Gamma |-- l is (TY_Ref T) ->
+    mt / Gamma |-- r is T ->
+    mt / Gamma |-- (TM_Asg l r) is TY_Void
+
+  where "mt / Gamma '|--' t 'is' T" := (well_typed_term mt Gamma t T).
